# baseURI: http://www.w3.org/ns/sosa/sampling
# imports: http://www.w3.org/2004/02/skos/core
# imports: http://www.w3.org/ns/sosa/

@prefix : <http://www.w3.org/ns/sosa/sampling/> .
@prefix owl: <http://www.w3.org/2002/07/owl#> .
@prefix rdf: <http://www.w3.org/1999/02/22-rdf-syntax-ns#> .
@prefix rdfs: <http://www.w3.org/2000/01/rdf-schema#> .
@prefix sampling: <http://www.w3.org/ns/sosa/sampling/> .
@prefix schema: <http://schema.org/> .
@prefix skos: <http://www.w3.org/2004/02/skos/core#> .
@prefix xsd: <http://www.w3.org/2001/XMLSchema#> .

<http://www.w3.org/ns/sosa/hasFeatureOfInterest>
  schema:domainIncludes sampling:Sampling ;
.
<http://www.w3.org/ns/sosa/hosts>
  schema:rangeIncludes sampling:Sampler ;
.
<http://www.w3.org/ns/sosa/resultTime>
  schema:domainIncludes sampling:Sampling ;
.
<http://www.w3.org/ns/sosa/sampling>
  rdf:type owl:Ontology ;
  owl:imports <http://www.w3.org/2004/02/skos/core> ;
  owl:imports <http://www.w3.org/ns/sosa/> ;
  owl:versionInfo "Created with TopBraid Composer" ;
.
sampling:RelationshipNature
  rdf:type owl:Class ;
  rdfs:comment "Members of this class indicate the nature of a relationship between two samples"@en ;
  rdfs:label "Nature of relationship (between samples)"@en ;
  rdfs:subClassOf skos:Concept ;
.
sampling:SampleRelationship
  rdf:type owl:Class ;
  rdfs:comment "Members of this class represent a relationship between a sample and another"@en ;
  rdfs:label "Sample relationship"@en ;
.
sampling:Sampler
  rdf:type rdfs:Class ;
  rdf:type owl:Class ;
  rdfs:comment "A device that is used by, or implements, a (Sampling) Procedure to create or transform one or more samples."@en ;
  rdfs:label "Sampling device"@en ;
  skos:definition "A device that is used by, or implements, an (Sampling) Procedure to create or transform one or more samples."@en ;
  skos:example "Ball mill"@en ;
  skos:example "Diamond drill"@en ;
  skos:example "Hammer"@en ;
  skos:example "Hypodermic syringe and needle"@en ;
  skos:example "Image sensor"@en ;
  skos:example "Seive stack"@en ;
  skos:example "Soil auger"@en ;
.
sampling:Sampling
  rdf:type rdfs:Class ;
  rdf:type owl:Class ;
  rdfs:comment "A Sampling activity carries out a (Sampling) Procedure to create or transform one or more samples."@en ;
  rdfs:label "Sampling activity"@en ;
  skos:definition "A Sampling activity carries out a (Sampling) Procedure to create or transform one or more samples."@en ;
  skos:example "Crushing a rock sample in a ball mill."@en ;
  skos:example "Digging a pit through a soil sequence."@en ;
  skos:example "Dividing a field site into quadrats."@en ;
  skos:example "Drawing blood from a patient."@en ;
  skos:example "Drilling an observation well."@en ;
  skos:example "Establishing a station for environmental monitoring."@en ;
  skos:example "Registering an image of the landscape."@en ;
  skos:example "Seiving a powder to separate the subset finer than 100-mesh."@en ;
  skos:example "Selecting a subset of a population."@en ;
  skos:example "Splitting a piece of drill-core to create two new samples."@en ;
  skos:example "Taking a diamond-drill core from a rock outcrop."@en ;
.
sampling:hasResultingSample
  rdf:type owl:ObjectProperty ;
  schema:domainIncludes sampling:Sampling ;
  schema:rangeIncludes <http://www.w3.org/ns/sosa/Sample> ;
  rdfs:comment "Relation linking a SamplingActivity and the new Sample created as a result."@en ;
  rdfs:label "has resulting sample"@en ;
  owl:inverseOf sampling:isSamplingResultOf ;
  skos:definition "Relation linking a SamplingActivity and the new Sample created as a result."@en ;
.
sampling:hasSampleRelationship
  rdf:type owl:ObjectProperty ;
  schema:domainIncludes <http://www.w3.org/ns/sosa/Sample> ;
  schema:rangeIncludes sampling:SampleRelationship ;
  rdfs:comment "Links a sample to a sample relationship (which links to a related sample)"@en ;
  rdfs:label "has sample relationship"@en ;
.
sampling:isSamplingResultOf
  rdf:type owl:ObjectProperty ;
  owl:inverseOf sampling:hasResultingSample ;
.
sampling:natureOfRelationship
  rdf:type owl:ObjectProperty ;
  schema:domainIncludes sampling:SampleRelationship ;
  schema:rangeIncludes sampling:RelationshipNature ;
  rdfs:comment "Links a SampleRelationship to an indication of the nature of the relationship"@en ;
  rdfs:label "nature of (sample) relationship"@en ;
.
sampling:performedSampling
  rdf:type owl:ObjectProperty ;
  owl:inverseOf sampling:sampledBy ;
.
sampling:relatedSample
  rdf:type owl:ObjectProperty ;
  schema:domainIncludes sampling:SampleRelationship ;
  schema:rangeIncludes <http://www.w3.org/ns/sosa/Sample> ;
  rdfs:comment "Links a sample relationship to the related sample"@en ;
  rdfs:label "related sample"@en ;
.
sampling:sampledBy
  rdf:type owl:ObjectProperty ;
  schema:domainIncludes sampling:Sampling ;
  schema:rangeIncludes sampling:Sampler ;
  rdfs:comment "Relation linking an SamplingActivity to the SamplingDevice that made that SamplingActivity."@en ;
  rdfs:label "sampled by"@en ;
  owl:inverseOf sampling:performedSampling ;
  skos:definition "Relation linking an SamplingActivity to the SamplingDevice that made that SamplingActivity."@en ;
.
<http://www.w3.org/ns/sosa/usedProcedure>
  schema:domainIncludes sampling:Sampling ;
  rdfs:comment "or to a re-usable Procedure used in a SamplingActivity" ;
  skos:definition "or to a re-usable Procedure used in a SamplingActivity" ;
.
