# baseURI: http://www.w3.org/ns/sosa/sampling
# imports: http://purl.org/dc/elements/1.1/
# imports: http://www.w3.org/2004/02/skos/core
# imports: http://www.w3.org/ns/sosa/

@prefix : <http://www.w3.org/ns/sosa/sampling/> .
@prefix dcterms: <http://purl.org/dc/terms/> .
@prefix owl: <http://www.w3.org/2002/07/owl#> .
@prefix rdf: <http://www.w3.org/1999/02/22-rdf-syntax-ns#> .
@prefix rdfs: <http://www.w3.org/2000/01/rdf-schema#> .
@prefix sampling: <http://www.w3.org/ns/sosa/sampling/> .
@prefix schema: <http://schema.org/> .
@prefix skos: <http://www.w3.org/2004/02/skos/core#> .
@prefix xsd: <http://www.w3.org/2001/XMLSchema#> .

<http://www.w3.org/ns/sosa/hasFeatureOfInterest>
  schema:domainIncludes sampling:SamplingActivity ;
.
<http://www.w3.org/ns/sosa/hosts>
  schema:rangeIncludes sampling:SamplingDevice ;
.
<http://www.w3.org/ns/sosa/resultTime>
  schema:domainIncludes sampling:SamplingActivity ;
.
<http://www.w3.org/ns/sosa/sampling>
  rdf:type owl:Ontology ;
  dcterms:created "2017-02-15" ;
  dcterms:creator <http://orcid.org/0000-0002-3884-3420> ;
  dcterms:license <http://creativecommons.org/licenses/by/4.0/> ;
  rdfs:comment "Proposal for extension to SOSA to support basic description of sampling activities."@en ;
  rdfs:label "Sampling extension of SOSA" ;
  owl:imports <http://purl.org/dc/elements/1.1/> ;
  owl:imports <http://www.w3.org/2004/02/skos/core> ;
  owl:imports <http://www.w3.org/ns/sosa/> ;
.
sampling:SamplingActivity
  rdf:type rdfs:Class ;
  rdf:type owl:Class ;
  rdfs:comment "A SamplingActivity carries out an (Sampling) Procedure to create or transform one or more samples."@en ;
  rdfs:label "Sampling Activity"@en ;
  skos:definition "A SamplingActivity carries out an (Sampling) Procedure to create or transform one or more samples."@en ;
  skos:example "Crushing a rock sample in a ball mill."@en ;
  skos:example "Digging a pit through a soil sequence."@en ;
  skos:example "Dividing a field site into quadrats."@en ;
  skos:example "Drawing blood from a patient."@en ;
  skos:example "Drilling an observation well."@en ;
  skos:example "Establishing a station for environmental monitoring."@en ;
  skos:example "Registering an image of the landscape."@en ;
  skos:example "Seiving a powder to separate the subset finer than 100-mesh."@en ;
  skos:example "Selecting a subset of a population."@en ;
  skos:example "Splitting a piece of drill-core to create two new samples."@en ;
  skos:example "Taking a diamond-drill core from a rock outcrop."@en ;
.
sampling:SamplingDevice
  rdf:type rdfs:Class ;
  rdf:type owl:Class ;
  rdfs:comment "A device that is used by, or implements, an (Sampling) Procedure to create or transform one or more samples."@en ;
  rdfs:label "Sampling Device"@en ;
  skos:definition "A device that is used by, or implements, an (Sampling) Procedure to create or transform one or more samples."@en ;
  skos:example "Ball mill."@en ;
  skos:example "Diamond drill."@en ;
  skos:example "Hammer."@en ;
  skos:example "Hypodermic syringe and needle."@en ;
  skos:example "Image sensor."@en ;
  skos:example "Seive stack."@en ;
  skos:example "Soil auger."@en ;
.
sampling:hasResultingSample
  rdf:type owl:ObjectProperty ;
  schema:domainIncludes sampling:SamplingActivity ;
  schema:rangeIncludes <http://www.w3.org/ns/sosa/Sample> ;
  rdfs:comment "Relation linking a SamplingActivity and the new Sample created as a result."@en ;
  rdfs:label "has resulting sample"@en ;
  owl:inverseOf sampling:isSamplingResultOf ;
  skos:definition "Relation linking a SamplingActivity and the new Sample created as a result."@en ;
.
sampling:isSamplingResultOf
  rdf:type owl:ObjectProperty ;
.
sampling:performedSampling
  rdf:type owl:ObjectProperty ;
.
sampling:sampledBy
  rdf:type owl:ObjectProperty ;
  schema:domainIncludes sampling:SamplingActivity ;
  schema:rangeIncludes sampling:SamplingDevice ;
  rdfs:comment "Relation linking an SamplingActivity to the SamplingDevice that made that SamplingActivity."@en ;
  rdfs:label "sampled by"@en ;
  owl:inverseOf sampling:performedSampling ;
  skos:definition "Relation linking an SamplingActivity to the SamplingDevice that made that SamplingActivity."@en ;
.
<http://www.w3.org/ns/sosa/usedProcedure>
  schema:domainIncludes sampling:SamplingActivity ;
  rdfs:comment "or to a re-usable Procedure used in a SamplingActivity" ;
  skos:definition "or to a re-usable Procedure used in a SamplingActivity" ;
.
