# baseURI: http://www.w3.org/ns/sosa/

@prefix dc: <http://purl.org/dc/elements/1.1/> .
@prefix meta: <http://meta.schema.org/> .
@prefix ns: <http://creativecommons.org/ns#> .
@prefix owl: <http://www.w3.org/2002/07/owl#> .
@prefix rdf: <http://www.w3.org/1999/02/22-rdf-syntax-ns#> .
@prefix rdfs: <http://www.w3.org/2000/01/rdf-schema#> .
@prefix schema: <http://schema.org/> .
@prefix sosa: <http://www.w3.org/ns/sosa#> .
@prefix terms: <http://purl.org/dc/terms/> .
@prefix xhtm: <http://www.w3.org/1999/xhtml> .
@prefix xsd: <http://www.w3.org/2001/XMLSchema#> .

ns:license
  rdf:type owl:AnnotationProperty ;
.
meta:domainIncludes
  rdf:type owl:AnnotationProperty ;
.
meta:rangeIncludes
  rdf:type owl:AnnotationProperty ;
.
dc:creator
  rdf:type owl:AnnotationProperty ;
.
dc:date
  rdf:type owl:AnnotationProperty ;
.
dc:identifier
  rdf:type owl:AnnotationProperty ;
.
dc:rights
  rdf:type owl:AnnotationProperty ;
.
dc:source
  rdf:type owl:AnnotationProperty ;
.
dc:title
  rdf:type owl:AnnotationProperty ;
.
terms:created
  rdf:type owl:AnnotationProperty ;
.
terms:modified
  rdf:type owl:AnnotationProperty ;
.
rdfs:comment
  rdf:type owl:AnnotationProperty ;
.
rdfs:isDefinedBy
  rdf:type owl:AnnotationProperty ;
.
rdfs:label
  rdf:type owl:AnnotationProperty ;
.
rdfs:seeAlso
  rdf:type owl:AnnotationProperty ;
.
owl:topObjectProperty
  rdf:type owl:ObjectProperty ;
.
<http://www.w3.org/ns/sosa>
  rdfs:comment "Sensor Observation, Sample, and Actuator (SOSA) Ontology." ;
  rdfs:comment "This ontology is based on the SSN Ontology by the W3C Semantic Sensor Networks Incubator Group (SSN-XG), together with considerations from the W3C/OGC Spatial Data on the Web Working Group." ;
  rdfs:comment "This version is based on the horizontal/vertical modularization proposed in the W3C/OGC Spatial Data on the Web Working Group: http://w3c.github.io/sdw/ssn/#modularisation" ;
  rdfs:label "Sensor Observation, Sample, and Actuator (SOSA) Core Ontology" ;
.
sosa:Actuation
  rdf:type rdfs:Class ;
  rdf:type owl:Class ;
  rdfs:comment "An Actuation carries out an (Actuation) Procedure to change the state of the world using an Actuator."@en ;
  rdfs:label "Actuation"@en ;
.
sosa:Actuator
  rdf:type rdfs:Class ;
  rdf:type owl:Class ;
  rdfs:comment "A device that is used by, or implements, an (Actuation) Procedure that changes the state of the world."@en ;
  rdfs:label "Actuator"@en ;
.
sosa:FeatureOfInterest
  rdf:type rdfs:Class ;
  rdf:type owl:Class ;
  rdfs:comment "For example, when measuring the height of a tree, the height is the ObservedProperty, 20m may be the Result of the Observation, and the tree is the FeatureOfInterest." ;
  rdfs:comment "The feature whose ObservableProperty is being observed by a Sensor to arrive at a Result."@en ;
  rdfs:label "Feature Of Interest"@en ;
.
sosa:ObservableProperty
  rdf:type rdfs:Class ;
  rdf:type owl:Class ;
  rdfs:comment "An observable Quality of a Thing; typically a FeatureOfInterest."@en ;
  rdfs:label "Observable Property"@en ;
.
sosa:Observation
  rdf:type rdfs:Class ;
  rdf:type owl:Class ;
  rdfs:comment "Activity of carrying out an (Observation) Procedure to estimate or calculate a value of a Property of a FeatureOfInterest. Links to a Platform or Sensor to describe what made the Observation and how; links to an ObservableProperty to describe what the result is an estimate of, and to a FeatureOfInterest to detail what that property was associated with. The Result is the output."@en ;
  rdfs:label "Observation"@en ;
.
sosa:Platform
  rdf:type rdfs:Class ;
  rdf:type owl:Class ;
  rdfs:comment "A device, (computational) system, or agent (including humans). A platform carries at least one Sensor, Actuator, or Sampling Device to produce observations, actuations, or samples, by following a Procedure. In case of virtual sensors, a platform can be a computing system which hosts software implementations, e.g., simulations."@en ;
  rdfs:label "Platform"@en ;
.
sosa:Procedure
  rdf:type rdfs:Class ;
  rdf:type owl:Class ;
  rdfs:comment "A workflow, protocol, plan, algorithm, or computational method specifying how to make an Observation, create a Sample, or make a change to the state of the world (via an Actuator). A Procedure is re-usable, and might be involved in many observations, samplings, or actuations. It explains the steps to be carried out to arrive at reproducible results."@en ;
  rdfs:comment "Many observations may be created via the same Procedure the same way as many tables are assembled using the same instructions (as information objects, not their concrete realization)." ;
  rdfs:label "Procedure"@en ;
.
sosa:Result
  rdf:type rdfs:Class ;
  rdf:type owl:Class ;
  rdfs:comment "The Result of an Observation, Actuation, or Sampling. Such result can, for instance, store an observation's value via the hasValue property, e.g., the value for an ObservedProperty of some FeatureOfInterest such as 20m for the height of a tree."@en ;
  rdfs:label "Result"@en ;
.
sosa:Sample
  rdf:type rdfs:Class ;
  rdf:type owl:Class ;
  rdfs:comment "EXAMPLE A \"station\" is essentially an identifiable locality where a sensor system or Process may be deployed and an observation made. In the context of the observation model, it connotes the “world in the vicinity of the station”, so the observed properties relate to the physical medium at the station, and not to any physical artifact such as a mooring, buoy, benchmark, monument, well, etc." ;
  rdfs:comment "Feature on which Observations may be made, which is intended to be representative of a FeatureOfInterest that is not fully accessible."@en ;
  rdfs:comment "NOTE A transient sample, such as a ships-track or flight-line, might be identified and described, but is unlikely to be revisited exactly." ;
  rdfs:comment """Samples are artifacts of an observational strategy, and have no significant function outside of their role in the observation process. The characteristics of the samples themselves are of little interest, except perhaps to the manager of a sampling campaign.

A Sample is intended to sample some FatureOfInterest in an application domain, so there is an expectation of at least one sampledFeature property. However, in some cases the identity, and even the exact type, of the sampled feature may not be known when observations are made using the sampling features."""@en ;
  rdfs:label "Sample"@en ;
.
sosa:Sensor
  rdf:type rdfs:Class ;
  rdf:type owl:Class ;
  rdfs:comment "Device, agent (including humans), or software (simulation) involved in, or implementing, a (Sensing) Procedure. Sensors responds to a stimulus, e.g., a change in the environment, and generate a Result. Sensors can be mounted on Platforms, e.g., a modern smart phone hosts multiple sensors."@en ;
  rdfs:label "Sensor"@en ;
.
sosa:hasFeatureOfInterest
  rdf:type owl:ObjectProperty ;
  meta:domainIncludes sosa:Observation ;
  meta:rangeIncludes sosa:FeatureOfInterest ;
  meta:rangeIncludes sosa:Sample ;
  rdfs:comment "A relation between an Observation and the entity whose quality was observed. " ;
  rdfs:comment "For example, in an Observation of the weight of a person, the FeatureOfInterest is the person and the quality is weight." ;
  rdfs:label "has feature of interest"@en ;
  owl:inverseOf sosa:isFeatureOfInterestOf ;
.
sosa:hasResult
  rdf:type owl:ObjectProperty ;
  meta:domainIncludes sosa:Observation ;
  meta:rangeIncludes sosa:Result ;
  rdfs:comment "Relation linking an Observation and a Sensor or Actuator and a Result, which contains a value representing the value associated with the observed Property." ;
  rdfs:label "has result"@en ;
  owl:inverseOf sosa:isResultOf ;
.
sosa:hasSample
  rdf:type owl:ObjectProperty ;
  meta:domainIncludes sosa:FeatureOfInterest ;
  meta:rangeIncludes sosa:Sample ;
  rdfs:comment "Relation between a FeatureOfInterest and the Sample used to represent it." ;
  rdfs:label "has sample"@en ;
  owl:inverseOf sosa:isSampleOf ;
.
sosa:hasValue
  rdf:type owl:DatatypeProperty ;
  rdfs:comment "The value of a Result, e.g., 23 or true." ;
  rdfs:label "has value"@en ;
.
sosa:hostedBy
  rdf:type owl:ObjectProperty ;
  meta:domainIncludes sosa:Actuator ;
  meta:domainIncludes sosa:Sensor ;
  meta:rangeIncludes sosa:Platform ;
  rdfs:comment "Relation between a Sensor or Actuator and the Platform that it is mounted on or hosted by." ;
  rdfs:label "hosted by"@en ;
  owl:inverseOf sosa:hosts ;
.
sosa:hosts
  rdf:type owl:ObjectProperty ;
  meta:domainIncludes sosa:Platform ;
  meta:rangeIncludes sosa:Actuator ;
  meta:rangeIncludes sosa:Sensor ;
  rdfs:comment "Relation between a Platform and a Sensor or Actuator (or SamplingDevice) hosted or mounted on it." ;
  rdfs:label "hosts"@en ;
  owl:inverseOf sosa:hostedBy ;
.
sosa:invokedBy
  rdf:type owl:ObjectProperty ;
  meta:domainIncludes sosa:Actuation ;
  meta:rangeIncludes sosa:Actuator ;
  rdfs:comment "Relation linking an Actuation to the Actuator that made that Actuation." ;
  rdfs:label "invoked by"@en ;
  owl:inverseOf sosa:invokes ;
.
sosa:invokes
  rdf:type owl:ObjectProperty ;
  meta:domainIncludes sosa:Actuator ;
  meta:rangeIncludes sosa:Actuation ;
  rdfs:comment "Relation between an Actuator and the Actuation it has made." ;
  rdfs:label "invokes"@en ;
.
sosa:isFeatureOfInterestOf
  rdf:type owl:ObjectProperty ;
  meta:domainIncludes sosa:FeatureOfInterest ;
  meta:rangeIncludes sosa:Observation ;
  rdfs:comment "A relation between a FeatureOfInterest and an Observation about it." ;
  rdfs:label "is feature of interest of"@en ;
  owl:inverseOf sosa:hasFeatureOfInterest ;
.
sosa:isObservedBy
  rdf:type owl:ObjectProperty ;
  meta:domainIncludes sosa:ObservableProperty ;
  meta:rangeIncludes sosa:Sensor ;
  rdfs:comment "Relation between an ObservableProperty and the Sensor able to observe it." ;
  rdfs:label "is observed by"@en ;
  owl:inverseOf sosa:observes ;
.
sosa:isResultOf
  rdf:type owl:ObjectProperty ;
  meta:domainIncludes sosa:Result ;
  meta:rangeIncludes sosa:Observation ;
  rdfs:comment "Relation linking a Result to the Observation that created it." ;
  rdfs:label "is result of"@en ;
  owl:inverseOf sosa:hasResult ;
.
sosa:isSampleOf
  rdf:type owl:ObjectProperty ;
  meta:domainIncludes sosa:Sample ;
  meta:rangeIncludes sosa:FeatureOfInterest ;
  rdfs:comment "Relation from a Sample to the FeatureOfInterest that it is intended to be representative of." ;
  rdfs:label "is sample of"@en ;
  owl:inverseOf sosa:hasSample ;
.
sosa:madeObservation
  rdf:type owl:ObjectProperty ;
  meta:domainIncludes sosa:Sensor ;
  meta:rangeIncludes sosa:Observation ;
  rdfs:comment "Relation between a Sensor and an Observations it has made." ;
  rdfs:label "made observation"@en ;
.
sosa:observedProperty
  rdf:type owl:ObjectProperty ;
  meta:domainIncludes sosa:Observation ;
  meta:rangeIncludes sosa:ObservableProperty ;
  rdfs:comment "Relation linking an Observation to the Property that was observed. The observedProperty should be a Property (hasProperty) of the FeatureOfInterest (linked by featureOfInterest) of this observation." ;
  rdfs:label "observed property"@en ;
.
sosa:observes
  rdf:type owl:ObjectProperty ;
  meta:domainIncludes sosa:Sensor ;
  meta:rangeIncludes sosa:ObservableProperty ;
  rdfs:comment "Relation between a Sensor and an ObservableProperty." ;
  rdfs:label "observes"@en ;
  owl:inverseOf sosa:isObservedBy ;
.
sosa:phenomenonTime
  rdf:type owl:ObjectProperty ;
  meta:domainIncludes sosa:Actuation ;
  meta:domainIncludes sosa:Observation ;
  rdfs:comment "The time that the Result of an Observation/Actuation applies to the FeatureOfInterest. Not necessarily the same as the result-time. May be an interval or an instant, or some other compound temporal entity. " ;
  rdfs:label "phenomenon time"@en ;
.
sosa:resultTime
  rdf:type owl:DatatypeProperty ;
  meta:domainIncludes sosa:Actuation ;
  meta:domainIncludes sosa:Observation ;
  rdfs:comment "The result time is the time when the Observation or Actuation act was completed." ;
  rdfs:label "result time"@en ;
  rdfs:range xsd:dateTime ;
.
sosa:usedProcess
  rdf:type owl:ObjectProperty ;
  meta:domainIncludes sosa:Actuation ;
  meta:domainIncludes sosa:Observation ;
  meta:rangeIncludes sosa:Procedure ;
  rdfs:comment "Relation to link to a re-usable Process used in making an Observation or Actuation. Typically a sensor or sensor-system, algorithm, computational Process." ;
  rdfs:label "used process"@en ;
.
<http://www.w3.org/ns/sosa/>
  rdf:type owl:Ontology ;
.
